Redoing locally nameless STLC, with more Dafny experience.
Works like a charm so far.

StlcLn.dfy
@@ -5,6 +5,20 @@
 // https://github.com/namin/coq-sandbox/blob/master/STLC.v
 
 datatype atom = a(i: nat);
+function max(s: seq<atom>, start: int): int
+  ensures max(s, start)>=start;
+  ensures forall x:nat :: a(x) in s ==> x<=max(s, start);
+{
+  if (s == []) then start
+  else if (s[0].i <= start) then max(s[1..], start)
+  else max(s[1..], s[0].i)
+}
+function fresh_from(ids: seq<atom>): atom
+  ensures fresh_from(ids) !in ids;
+  ensures fresh_from(ids).i>0;
+{
+  a(max(ids, 0)+1)
+}
 
 datatype typ = typ_base | typ_arrow(typ, typ);
 
@@ -27,65 +41,38 @@ ghost method example_subst1(Y: atom, Z: atom)
   assert subst(Y, fvar(Z), app(bvar(0), fvar(Y))) == app(bvar(0), fvar(Z));
 }
 
-function fv(e: exp) : set<atom>
+ghost method lemma_subst_eq_var(x: atom, u: exp)
+  ensures subst(x, u, fvar(x)) == u;
+{
+}
+
+ghost method lemma_subst_neq_var(x: atom, y: atom, u: exp)
+  requires y != x;
+  ensures subst(x, u, fvar(y)) == fvar(y);
+{
+}
+
+function fv(e: exp) : seq<atom>
   decreases e;
 {
   match e
-  case bvar(i) => {}
-  case fvar(x) => {x}
+  case bvar(i) => []
+  case fvar(x) => [x]
   case abs(e1) => fv(e1)
   case app(e1, e2) => fv(e1) + fv(e2)
 }
 
 ghost method lemma_subst_fresh(x: atom, e: exp, u: exp)
-  requires !(x in fv(e));
+  requires x !in fv(e);
   ensures subst(x, u, e) == e;
 {
 }
 
-function open_rec(k: nat, u: exp, e: exp): exp
-  decreases e;
+ghost method lemma_subst_notin_fv(x: atom, y: atom, u: exp, e: exp)
+  requires x !in fv(e);
+  requires x !in fv(u);
+  ensures x !in fv(subst(y, u, e));
 {
-  match e
-  case bvar(i) => if k==i then u else bvar(i)
-  case fvar(x) => fvar(x)
-  case abs(e1) => abs(open_rec(k+1, u, e1))
-  case app(e1, e2) => app(open_rec(k, u, e1), open_rec(k, u, e2))
-}
-
-function open(e: exp, u: exp): exp
-{
-  open_rec(0, u, e)
-}
-
-function open_rec_a(k: nat, a: atom, e: exp): exp
-  decreases e;
-  ensures size(e) == size(open_rec_a(k, a, e));
-  ensures open_rec_a(k, a, e) == open_rec(k, fvar(a), e);
-{
-  match e
-  case bvar(i) => if k==i then fvar(a) else bvar(i)
-  case fvar(x) => fvar(x)
-  case abs(e1) => abs(open_rec_a(k+1, a, e1))
-  case app(e1, e2) => app(open_rec_a(k, a, e1), open_rec_a(k, a, e2))
-}
-
-function open_a(e: exp, a: atom): exp
-  ensures size(e) == size(open_a(e, a));
-  ensures open_a(e, a) == open(e, fvar(a));
-{
-  open_rec_a(0, a, e)
-}
-
-ghost method example_open(Y: atom)
-  ensures open(app(abs(app(bvar(1), bvar(0))), bvar(0)), fvar(Y)) ==
-               app(abs(app(fvar(Y), bvar(0))), fvar(Y));
-{
-  assert open_rec(1, fvar(Y), bvar(1)) == fvar(Y);
-  assert open_rec(1, fvar(Y), bvar(0)) == bvar(0);
-  assert open_rec(0, fvar(Y), abs(app(bvar(1), bvar(0)))) ==
-                              abs(app(fvar(Y), bvar(0)));
-  assert open_rec(0, fvar(Y), bvar(0)) == fvar(Y);
 }
 
 function size(e: exp): nat
@@ -101,415 +88,147 @@ function size(e: exp): nat
   case app(e1, e2) => 1 + size(e1) + size(e2)
 }
 
-copredicate lc_fvar(e: exp)
-  requires e.fvar?;
+function open_rec(k: nat, u: exp, e: exp): exp
+  ensures u.fvar? ==> size(e) == size(open_rec(k, u, e));
+  decreases e;
 {
-  true
-}
-copredicate lc_abs(e: exp, L: seq<atom>)
-  requires e.abs?;
-{
-  forall x :: x !in L ==> lc(open_a(e.body, x), L)
-}
-copredicate lc_app(e: exp, L: seq<atom>)
-  requires e.app?;
-{
-  lc(e.f, L) && lc(e.arg, L)
-}
-copredicate lc(e: exp, L: seq<atom>)
-{
-  (e.fvar? && lc_fvar(e)) ||
-  (e.abs? && lc_abs(e, L)) ||
-  (e.app? && lc_app(e, L))
+  match e
+  case bvar(i) => if k==i then u else bvar(i)
+  case fvar(x) => fvar(x)
+  case abs(e1) => abs(open_rec(k+1, u, e1))
+  case app(e1, e2) => app(open_rec(k, u, e1), open_rec(k, u, e2))
 }
 
-datatype option<T> = None | Some(get: T);
-datatype ev_lc = ev_lc_fvar | ev_lc_abs(sup: nat) | ev_lc_app(ev_f: ev_lc, ev_arg: ev_lc);
-function ev_lc_maxsup(ev: ev_lc, s: nat): nat
+function open(e: exp, u: exp): exp
+  ensures u.fvar? ==> size(e) == size(open(e, u));
 {
-  match ev
-  case ev_lc_fvar => s
-  case ev_lc_abs(sup) => if (sup <= s) then s else sup
-  case ev_lc_app(ev_f, ev_arg) => if (ev_lc_maxsup(ev_arg, s) <= ev_lc_maxsup(ev_f, s)) then ev_lc_maxsup(ev_f, s) else ev_lc_maxsup(ev_arg, s)
+  open_rec(0, u, e)
 }
-ghost method ev_lc_maxsup_prop(ev: ev_lc, r: nat)
-  requires ev_lc_maxsup(ev, r) <= r;
-  ensures ev.ev_lc_fvar? ==> r <= r;
-  ensures ev.ev_lc_app? ==> ev_lc_maxsup(ev.ev_f, r) <= r && ev_lc_maxsup(ev.ev_arg, r) <= r;
-  ensures ev.ev_lc_abs? ==> ev.sup <= r;
+
+ghost method example_open(Y: atom)
+  ensures open(app(abs(app(bvar(1), bvar(0))), bvar(0)), fvar(Y)) == app(abs(app(fvar(Y), bvar(0))), fvar(Y));
 {
+  calc == {
+    open(app(abs(app(bvar(1), bvar(0))), bvar(0)), fvar(Y));
+    open_rec(0, fvar(Y), app(abs(app(bvar(1), bvar(0))), bvar(0)));
+    app(open_rec(0, fvar(Y), abs(app(bvar(1), bvar(0)))), open_rec(0, fvar(Y), bvar(0)));
+    app(abs(open_rec(1, fvar(Y), app(bvar(1), bvar(0)))), open_rec(0, fvar(Y), bvar(0)));
+    app(abs(app(fvar(Y), bvar(0))), fvar(Y));
+  }
 }
-predicate is_ev_lc(e: exp, ev: ev_lc)
+
+predicate lc(e: exp)
+  ensures lc(e) ==> !e.bvar?;
   decreases size(e);
 {
-  match ev
-  case ev_lc_fvar => e.fvar?
-  case ev_lc_abs(sup) => e.abs? && build_ev_lc(open_a(e.body, a(sup)), sup).Some? && forall i :: i >= sup ==> build_ev_lc(open_a(e.body, a(i)), sup) == build_ev_lc(open_a(e.body, a(sup)), sup)
-  case ev_lc_app(ev_f, ev_arg) => e.app? && is_ev_lc(e.f, ev_f) && is_ev_lc(e.arg, ev_arg)
-}
-function build_ev_lc(e: exp, sup: nat): option<ev_lc>
-  decreases size(e);
-  ensures build_ev_lc(e, sup).Some? ==> ev_lc_maxsup(build_ev_lc(e, sup).get, sup) == sup;
-{
-  if (e.fvar?) then Some(ev_lc_fvar)
-  else if (e.abs? && build_ev_lc(open_a(e.body, a(sup)), sup).Some? && forall i :: i >= sup ==> build_ev_lc(open_a(e.body, a(i)), sup) == build_ev_lc(open_a(e.body, a(sup)), sup)) then Some(ev_lc_abs(sup))
-  else if (e.app? && build_ev_lc(e.f, sup).Some? && build_ev_lc(e.arg, sup).Some?) then Some(ev_lc_app(build_ev_lc(e.f, sup).get, build_ev_lc(e.arg, sup).get))
-  else None
-}
-ghost method built_ev_lc(e: exp, sup: nat)
-  requires build_ev_lc(e, sup).Some?;
-  ensures is_ev_lc(e, build_ev_lc(e, sup).get);
-  decreases size(e);
-{
-}
-ghost method can_build_ev_lc(e: exp, sup: nat, ev: ev_lc)
-  requires ev_lc_maxsup(ev, sup) <= sup;
-  requires is_ev_lc(e, ev);
-  ensures build_ev_lc(e, sup).Some?;
-{
-  if (e.abs?) {
-    assert ev.sup <= sup;
-    build_ev_lc_bigger(open_a(e.body, a(sup)), ev.sup, sup);
-    built_ev_lc(open_a(e.body, a(sup)), sup);
-    var ev_body :=  build_ev_lc(open_a(e.body, a(sup)), sup).get;
-    forall (i | i >= sup)
-      ensures build_ev_lc(open_a(e.body, a(i)), sup) == Some(ev_body);
-    {
-      build_ev_lc_bigger(open_a(e.body, a(i)), ev.sup, sup);
-      build_ev_lc_bigger_open(e.body, i, ev.sup, sup, build_ev_lc(open_a(e.body, a(i)), ev.sup).get, ev_body);
-    }
-  }
-  if (e.app?) {
-    can_build_ev_lc(e.f, sup, ev.ev_f);
-    can_build_ev_lc(e.arg, sup, ev.ev_arg);
-  }
-}
-ghost method build_ev_lc_bigger_open(e: exp, i: nat, sup: nat, sup': nat, ev: ev_lc, ev': ev_lc)
-  requires i >= sup';
-  requires build_ev_lc(open_a(e, a(i)), sup) == Some(ev);
-  requires build_ev_lc(open_a(e, a(sup)), sup) == Some(ev);
-  requires build_ev_lc(open_a(e, a(sup')), sup') == Some(ev');
-  requires build_ev_lc(open_a(e, a(i)), sup').Some?;
-  ensures build_ev_lc(open_a(e, a(i)), sup') == Some(ev');
-{
-  if (e.abs?) {
-    assert ev' == ev_lc_abs(sup');
-  }
-  if (e.app?) {
-    build_ev_lc_bigger_open(e.f, i, sup, sup', ev.ev_f, ev'.ev_f);
-    build_ev_lc_bigger_open(e.arg, i, sup, sup', ev.ev_arg, ev'.ev_arg);
-  }
-}
-ghost method build_ev_lc_bigger(e: exp, sup: nat, sup': nat)
-  requires build_ev_lc(e, sup).Some?;
-  requires sup' >= sup;
-  ensures build_ev_lc(e, sup').Some?;
-  decreases size(e);
-{
-  if (e.abs?) {
-    var evL := build_ev_lc(e, sup).get;
-    assert build_ev_lc(open_a(e.body, a(sup)), sup).Some?;
-    assert forall i :: i >= sup ==> build_ev_lc(open_a(e.body, a(i)), sup) == build_ev_lc(open_a(e.body, a(sup)), sup);
-    assert forall i :: i >= sup' ==> build_ev_lc(open_a(e.body, a(i)), sup) == build_ev_lc(open_a(e.body, a(sup)), sup);
-    forall (i | i >= sup')
-      ensures build_ev_lc(open_a(e.body, a(sup')), sup').Some?;
-      ensures build_ev_lc(open_a(e.body, a(i)), sup') == build_ev_lc(open_a(e.body, a(sup')), sup');
-    {
-      build_ev_lc_bigger(open_a(e.body, a(i)), sup, sup');
-      build_ev_lc_bigger_open(e.body, i, sup, sup', build_ev_lc(open_a(e.body, a(sup)), sup).get,  build_ev_lc(open_a(e.body, a(sup')), sup').get);
-    }
-  }
-}
-
-ghost method equiv_ev_lc_subst_open(e: exp, x: atom, u: exp, i: nat, sup: nat)
-  requires x.i < sup;
-  requires i >= sup;
-  requires build_ev_lc(subst(x, u, open(e, fvar(a(i)))), sup).Some?;
-  requires build_ev_lc(subst(x, u, open(e, fvar(a(sup)))), sup).Some?;
-  ensures build_ev_lc(subst(x, u, open(e, fvar(a(i)))), sup) == build_ev_lc(subst(x, u, open(e, fvar(a(sup)))), sup);
-{
-  if (e.abs?) {
-
-  }
-  else if (e.app?) {
-    equiv_ev_lc_subst_open(e.f, x, u, i, sup);
-    equiv_ev_lc_subst_open(e.arg, x, u, i, sup);
-  }
-  else if (e.fvar?) {
-
-  }
-  else if (e.bvar?) {
-
-  }
-}
-
-ghost method equiv_ev_lc_subst(e: exp, x: atom, y: atom, z: atom, sup: nat)
-  requires x.i < sup;
-  requires build_ev_lc(subst(x, fvar(y), e), sup).Some?;
-  ensures build_ev_lc(subst(x, fvar(z), e), sup) == build_ev_lc(subst(x, fvar(y), e), sup);
-  decreases size(e);
-{
-  if (e.abs?) {
-    assert build_ev_lc(open_a(subst(x, fvar(y), e).body, a(sup)), sup).Some?;
-    assert open_a(subst(x, fvar(y), e).body, a(sup)) == open(subst(x, fvar(y), e).body, fvar(a(sup)));
-    assert open(subst(x, fvar(y), e).body, fvar(a(sup))) == open(subst(x, fvar(y), e.body), fvar(a(sup)));
-    lemma_subst_open_var'(x, a(sup), fvar(y), e.body, ev_lc_fvar);
-    assert open(subst(x, fvar(y), e.body), fvar(a(sup))) == subst(x, fvar(y), open(e.body, fvar(a(sup))));
-
-    equiv_ev_lc_subst(open_a(e.body, a(sup)), x, y, z, sup);
-    assert build_ev_lc(subst(x, fvar(z), open(e.body, fvar(a(sup)))), sup) == build_ev_lc(subst(x, fvar(y), open(e.body, fvar(a(sup)))), sup);
-
-    lemma_subst_open_var'(x, a(sup), fvar(z), e.body, ev_lc_fvar);
-    assert open(subst(x, fvar(z), e.body), fvar(a(sup))) == subst(x, fvar(z), open(e.body, fvar(a(sup))));
-    assert open(subst(x, fvar(z), e).body, fvar(a(sup))) == open(subst(x, fvar(z), e.body), fvar(a(sup)));
-    assert open_a(subst(x, fvar(z), e).body, a(sup)) == open(subst(x, fvar(z), e).body, fvar(a(sup)));
-    assert build_ev_lc(open_a(subst(x, fvar(z), e).body, a(sup)), sup).Some?;
-
-    assert forall i :: i >= sup ==> build_ev_lc(open_a(subst(x, fvar(y), e).body, a(i)), sup) == build_ev_lc(open_a(subst(x, fvar(y), e).body, a(sup)), sup);
-    forall (i | i >= sup)
-      ensures build_ev_lc(subst(x, fvar(z), open(e.body, fvar(a(i)))), sup) == build_ev_lc(subst(x, fvar(y), open(e.body, fvar(a(i)))), sup);
-      ensures build_ev_lc(subst(x, fvar(z), open(e.body, fvar(a(i)))), sup) == build_ev_lc(subst(x, fvar(z), open(e.body, fvar(a(sup)))), sup);
-      ensures build_ev_lc(subst(x, fvar(y), open(e.body, fvar(a(i)))), sup) == build_ev_lc(subst(x, fvar(z), open(e.body, fvar(a(i)))), sup);
-      ensures open(subst(x, fvar(y), e.body), fvar(a(i))) == subst(x, fvar(y), open(e.body, fvar(a(i))));
-      ensures open(subst(x, fvar(z), e.body), fvar(a(i))) == subst(x, fvar(z), open(e.body, fvar(a(i))));
-    {
-      assert build_ev_lc(open_a(subst(x, fvar(y), e).body, a(i)), sup).Some?;
-      assert open_a(subst(x, fvar(y), e).body, a(i)) == open(subst(x, fvar(y), e).body, fvar(a(i)));
-      assert open(subst(x, fvar(y), e).body, fvar(a(i))) == open(subst(x, fvar(y), e.body), fvar(a(i)));
-      lemma_subst_open_var'(x, a(i), fvar(y), e.body, ev_lc_fvar);
-      assert open(subst(x, fvar(y), e.body), fvar(a(i))) == subst(x, fvar(y), open(e.body, fvar(a(i))));
-
-      equiv_ev_lc_subst(open_a(e.body, a(i)), x, y, z, sup);
-      assert build_ev_lc(subst(x, fvar(z), open(e.body, fvar(a(i)))), sup) == build_ev_lc(subst(x, fvar(y), open(e.body, fvar(a(i)))), sup);
-
-      lemma_subst_open_var'(x, a(i), fvar(z), e.body, ev_lc_fvar);
-      assert open(subst(x, fvar(z), e.body), fvar(a(i))) == subst(x, fvar(z), open(e.body, fvar(a(i))));
-      assert open(subst(x, fvar(z), e).body, fvar(a(i))) == open(subst(x, fvar(z), e.body), fvar(a(i)));
-      assert open_a(subst(x, fvar(z), e).body, a(i)) == open(subst(x, fvar(z), e).body, fvar(a(i)));
-      assert build_ev_lc(open_a(subst(x, fvar(z), e).body, a(i)), sup).Some?;
-    }
-    assert build_ev_lc(subst(x, fvar(z), e), sup) == Some(ev_lc_abs(sup));
-    assert build_ev_lc(subst(x, fvar(y), e), sup) == Some(ev_lc_abs(sup));
-  }
-  else if (e.app?) {
-
-  }
-  else if (e.fvar?) {
-
-  }
-  else if (e.bvar?) {
-
-  }
+  e.fvar? ||
+  (e.abs? && forall x :: x !in fv(e) ==> lc(open(e.body, fvar(x)))) ||
+  (e.app? && lc(e.f) && lc(e.arg))
 }
 
 ghost method lemma_open_rec_lc_core(e: exp, j: nat, v: exp, i: nat, u: exp)
   requires i != j;
   requires open_rec(j, v, e) == open_rec(i, u, open_rec(j, v, e));
   ensures e == open_rec(i, u, e);
-  decreases e;
 {
   if (e.abs?) {
     lemma_open_rec_lc_core(e.body, j+1, v, i+1, u);
   }
 }
 
-ghost method notin(L: seq<atom>) returns (r: atom)
-  ensures r !in L;
-  ensures forall j :: j > r.i ==> a(j) !in L;
-  decreases L;
-{
-  var sup:nat := 0;
-  var i: nat := 0;
-  while (i < |L|)
-    invariant 0 <= i <= |L|;
-    invariant forall j :: 0 <= j < i ==> L[j].i <= sup;
-  {
-      if (L[i].i > sup) {
-        sup := L[i].i;
-      }
-      i := i + 1;
-    }
-  r := a(sup+1);
-}
-
-ghost method lemma_open_rec_lc(k: nat, u: exp, e: exp, L: seq<atom>)
-  requires lc(e, L);
+ghost method lemma_open_rec_lc(k: nat, u: exp, e: exp)
+  requires lc(e);
   ensures e == open_rec(k, u, e);
   decreases size(e);
 {
   if (e.abs?) {
-    var x := notin(L);
-    assert lc_abs(e, L);
-    assert lc(open_a(e.body, x), L);
-    lemma_open_rec_lc(k+1, u, open_a(e.body, x), L);
-    assert open_rec(0, fvar(x), e.body) == open_rec(k+1, u, open_rec(0, fvar(x), e.body));
+    assert open_rec(k, u, e) == abs(open_rec(k+1, u, e.body));
+    var x := fresh_from(fv(e));
+    lemma_open_rec_lc(k+1, u, open(e.body, fvar(x)));
     lemma_open_rec_lc_core(e.body, 0, fvar(x), k+1, u);
-    assert e.body == open_rec(k+1, u, e.body);
   }
 }
 
-ghost method lemma_open_rec_lc'(k: nat, u: exp, e: exp, ev_lc_e: ev_lc)
-  requires is_ev_lc(e, ev_lc_e);
+ghost method lemma_subst_open_rec(e1: exp, e2: exp, u: exp, x: atom, k: nat)
+  requires lc(u);
+  ensures subst(x, u, open_rec(k, e2, e1)) == open_rec(k, subst(x, u, e2), subst(x, u, e1));
+{
+  if (e1.fvar?) {
+    if (e1.x==x) {
+      lemma_open_rec_lc(k, subst(x, u, e2), u);
+    }
+  }
+}
+
+ghost method lemma_subst_open_var(x: atom, y: atom, u: exp, e: exp)
+  requires y != x;
+  requires lc(u);
+  ensures open(subst(x, u, e), fvar(y)) == subst(x, u, open(e, fvar(y)));
+{
+  lemma_subst_open_rec(e, fvar(y), u, x, 0);
+}
+
+ghost method lemma_subst_intro_core(x: atom, u: exp, e: exp, k: nat)
+  requires x !in fv(e);
+  ensures open_rec(k, u, e) == subst(x, u, open_rec(k, fvar(x), e));
+{
+}
+
+ghost method lemma_subst_intro(x: atom, u: exp, e: exp)
+  requires x !in fv(e);
+  ensures open(e, u) == subst(x, u, open(e, fvar(x)));
+{
+  if (e.abs?) {
+    lemma_subst_intro_core(x, u, e.body, 1);
+  } else if (e.app?) {
+    lemma_subst_intro(x, u, e.f);
+    lemma_subst_intro(x, u, e.arg);
+  }
+}
+
+predicate lc_c(e: exp)
+  decreases size(e);
+{
+  e.fvar? ||
+  (e.abs? && forall L:seq<atom>, x :: x !in L ==> lc_c(open(e.body, fvar(x)))) ||
+  (e.app? && lc_c(e.f) && lc_c(e.arg))
+}
+
+ghost method lemma_open_rec_lc_c(k: nat, u: exp, e: exp)
+  requires lc_c(e);
   ensures e == open_rec(k, u, e);
   decreases size(e);
 {
   if (e.abs?) {
-    var sup := ev_lc_e.sup;
-    assert build_ev_lc(open_a(e.body, a(sup)), sup).Some?;
-    var ev_body := build_ev_lc(open_a(e.body, a(sup)), sup).get;
-    assert forall i :: i >= sup ==> build_ev_lc(open_a(e.body, a(i)), sup) == build_ev_lc(open_a(e.body, a(sup)), sup);
-    built_ev_lc(open_a(e.body, a(sup)), sup);
-    lemma_open_rec_lc'(k+1, u, open_a(e.body, a(sup)), ev_body);
-    lemma_open_rec_lc_core(e.body, 0, fvar(a(sup)), k+1, u);
-  }
-  if (e.app?) {
-    lemma_open_rec_lc'(k, u, e.f, ev_lc_e.ev_f);
-    lemma_open_rec_lc'(k, u, e.arg, ev_lc_e.ev_arg);
+    assert open_rec(k, u, e) == abs(open_rec(k+1, u, e.body));
+    var x := fresh_from(fv(e));
+    lemma_open_rec_lc_c(k+1, u, open(e.body, fvar(x)));
+    lemma_open_rec_lc_core(e.body, 0, fvar(x), k+1, u);
   }
 }
 
-ghost method lemma_subst_open_rec(e1: exp, e2: exp, u: exp, x: atom, k: nat, L: seq<atom>)
-  requires lc(u, L);
+ghost method lemma_subst_open_rec_c(e1: exp, e2: exp, u: exp, x: atom, k: nat)
+  requires lc_c(u);
   ensures subst(x, u, open_rec(k, e2, e1)) == open_rec(k, subst(x, u, e2), subst(x, u, e1));
-  decreases e1;
 {
-  if (e1.fvar? && e1.x==x) {
-    lemma_open_rec_lc(k, subst(x, u, e2), u, L);
-  }
-  if (e1.abs?) {
-    lemma_subst_open_rec(e1.body, e2, u, x, k+1, L);
+  if (e1.fvar?) {
+    if (e1.x==x) {
+      lemma_open_rec_lc_c(k, subst(x, u, e2), u);
+    }
   }
 }
 
-ghost method lemma_subst_open_rec'(e1: exp, e2: exp, u: exp, x: atom, k: nat, ev_lc_u: ev_lc)
-  requires is_ev_lc(u, ev_lc_u);
-  ensures subst(x, u, open_rec(k, e2, e1)) == open_rec(k, subst(x, u, e2), subst(x, u, e1));
-  decreases e1;
-{
-  if (e1.fvar? && e1.x==x) {
-    lemma_open_rec_lc'(k, subst(x, u, e2), u, ev_lc_u);
-  }
-  if (e1.abs?) {
-    lemma_subst_open_rec'(e1.body, e2, u,  x, k+1, ev_lc_u);
-  }
-}
-
-ghost method lemma_subst_open_var(x: atom, y: atom, u: exp, e: exp, L: seq<atom>)
+ghost method lemma_subst_open_var_c(x: atom, y: atom, u: exp, e: exp)
   requires y != x;
-  requires lc(u, L);
+  requires lc_c(u);
   ensures open(subst(x, u, e), fvar(y)) == subst(x, u, open(e, fvar(y)));
 {
-  lemma_subst_open_rec(e, fvar(y), u, x, 0, L);
+  lemma_subst_open_rec_c(e, fvar(y), u, x, 0);
 }
 
-ghost method lemma_subst_open_var'(x: atom, y: atom, u: exp, e: exp, ev_lc_u: ev_lc)
-  requires y != x;
-  requires is_ev_lc(u, ev_lc_u);
-  ensures open(subst(x, u, e), fvar(y)) == subst(x, u, open(e, fvar(y)));
+ghost method lemma_subst_lc_c(x: atom, u: exp, e: exp)
+  requires lc_c(e);
+  requires lc_c(u);
+  requires lc_c(subst(x, u, e));
 {
-  lemma_subst_open_rec'(e, fvar(y), u, x, 0, ev_lc_u);
-}
-
-ghost method lemma_subst_lc(x: atom, u: exp, e: exp, L: seq<atom>)
-  requires x in L;
-  requires lc(e, L);
-  requires lc(u, L);
-  ensures lc(subst(x, u, e), L);
-  decreases size(e);
-{
-  if (e.abs?) {
-    assert lc_abs(e, L);
-    forall (y | y !in L)
-      ensures lc(open(subst(x, u, e.body), fvar(y)), L);
-    {
-      lemma_subst_lc(x, u, open_a(e.body, y), L);
-      assert open_a(e.body, y) == open(e.body, fvar(y));
-      assert lc(open(e.body, fvar(y)), L);
-      assert lc(subst(x, u, open(e.body, fvar(y))), L);
-      lemma_subst_open_var(x, y, u, e.body, L);
-      assert lc(open(subst(x, u, e.body), fvar(y)), L);
-    }
-    assert lc_abs(subst(x, u, e), L);
-    assert lc(subst(x, u, e), L);
-  }
-}
-
-ghost method lemma_subst_lc'(x: atom, u: exp, e: exp, ev_lc_e: ev_lc, ev_lc_u: ev_lc, sup: nat) returns (ret: ev_lc)
-  requires x.i < sup;
-  requires ev_lc_maxsup(ev_lc_e, sup) <= sup;
-  requires ev_lc_maxsup(ev_lc_u, sup) <= sup;
-  requires is_ev_lc(e, ev_lc_e);
-  requires is_ev_lc(u, ev_lc_u);
-  ensures is_ev_lc(subst(x, u, e), ret);
-  ensures build_ev_lc(subst(x, u, e), sup) == Some(ret);
-  decreases size(e);
-{
-  if (ev_lc_e.ev_lc_fvar? && e.x!=x) {
-    ret := ev_lc_e;
-    assert is_ev_lc(subst(x, u, e), ret);
-    assert build_ev_lc(subst(x, u, e), sup) == Some(ret);
-  }
-  if (ev_lc_e.ev_lc_fvar? && e.x==x) {
-    can_build_ev_lc(subst(x, u, e), sup, ev_lc_u);
-    ret := build_ev_lc(subst(x, u, e), sup).get;
-    built_ev_lc(subst(x, u, e), sup);
-    assert is_ev_lc(subst(x, u, e), ret);
-    assert build_ev_lc(subst(x, u, e), sup) == Some(ret);
-  }
-  if (ev_lc_e.ev_lc_abs?) {
-    build_ev_lc_bigger(e, ev_lc_e.sup, sup);
-    assert build_ev_lc(e, sup).Some?;
-
-    built_ev_lc(open_a(e.body, a(sup)), sup);
-    var ev_subst_body_sup := lemma_subst_lc'(x, u, open_a(e.body, a(sup)), build_ev_lc(open_a(e.body, a(sup)), sup).get, ev_lc_u, sup);
-    assert open_a(e.body, a(sup)) == open(e.body, fvar(a(sup)));
-    assert build_ev_lc(subst(x, u, open(e.body, fvar(a(sup)))), sup) == Some(ev_subst_body_sup);
-    lemma_subst_open_var'(x, a(sup), u, e.body, ev_lc_u);
-    assert open(subst(x, u, e.body), fvar(a(sup))) == subst(x, u, open(e.body, fvar(a(sup))));
-    assert build_ev_lc(open(subst(x, u, e.body), fvar(a(sup))), sup) == Some(ev_subst_body_sup);
-
-    forall (i | i >= sup)
-      ensures build_ev_lc(open(subst(x, u, e.body), fvar(a(i))), sup) == Some(ev_subst_body_sup);
-    {
-      built_ev_lc(open_a(e.body, a(i)), sup);
-      var ev_subst_body := lemma_subst_lc'(x, u, open_a(e.body, a(i)), build_ev_lc(open_a(e.body, a(i)), sup).get, ev_lc_u, sup);
-      assert open_a(e.body, a(i)) == open(e.body, fvar(a(i)));
-      assert build_ev_lc(subst(x, u, open(e.body, fvar(a(i)))), sup) == Some(ev_subst_body);
-      equiv_ev_lc_subst_open(e.body, x, u, i, sup);
-      assert build_ev_lc(subst(x, u, open(e.body, fvar(a(i)))), sup) == Some(ev_subst_body_sup);
-      lemma_subst_open_var'(x, a(i), u, e.body, ev_lc_u);
-      assert open(subst(x, u, e.body), fvar(a(i))) == subst(x, u, open(e.body, fvar(a(i))));
-      assert build_ev_lc(open(subst(x, u, e.body), fvar(a(i))), sup) == Some(ev_subst_body_sup);
-    }
-    assert build_ev_lc(subst(x, u, e), sup) == Some(ev_lc_abs(sup));
-    assert is_ev_lc(subst(x, u, e), ev_lc_abs(sup));
-    ret := ev_lc_abs(sup);
-    assert is_ev_lc(subst(x, u, e), ret);
-    assert build_ev_lc(subst(x, u, e), sup) == Some(ret);
-  }
-  if (ev_lc_e.ev_lc_app?) {
-    var ev_f := lemma_subst_lc'(x, u, e.f, ev_lc_e.ev_f, ev_lc_u, sup);
-    var ev_arg := lemma_subst_lc'(x, u, e.arg, ev_lc_e.ev_arg, ev_lc_u, sup);
-    ret := ev_lc_app(ev_f, ev_arg);
-    assert is_ev_lc(subst(x, u, e), ret);
-    assert build_ev_lc(subst(x, u, e), sup) == Some(ret);
-  }
-  assert is_ev_lc(subst(x, u, e), ret);
-  assert build_ev_lc(subst(x, u, e), sup) == Some(ret);
-}
-
-datatype env = Empty | Extend(a: atom, T: typ, r: env);
-
-function dom(ctx: env): seq<atom>
-{
-  match ctx
-  case Empty => []
-  case Extend(a, T, r) => [a] + dom(r)
-}
-
-predicate binds(a: atom, T: typ, ctx: env)
-{
-  match ctx
-  case Empty => false
-  case Extend(a', T', r) => if a==a' then T'==T else binds(a, T, r)
 }
